m2c_AppliedOperator'_symbol_builtin

minuska/theories/color.v
@@ -8,9 +8,6 @@ From CoLoR Require Import
     Term.Varyadic.VTerm
 .
 
-Print spec_syntax.Signature.
-Print VSignature.Signature.
-
 Inductive m2c_sig_symbols (Σ : spec_syntax.Signature) : Type :=
 | c_sym_symbol (s : @spec_syntax.symbol Σ)
 | c_sym_builtin_value
@@ -58,3 +55,165 @@ Definition m2c_sig
         (beq_m2c_sig_symbols Σ)
         (beq_m2c_sig_symbols_ok Σ)
 .
+
+Coercion m2c_sig : spec_syntax.Signature >-> VSignature.Signature.
+
+Print VTerm.term.
+
+Definition vterm_is_closed
+    {Σ : spec_syntax.Signature}
+    (t : VTerm.term Σ)
+    : Prop
+:= @VTerm.term_rect
+    Σ
+    (fun _ => Prop)
+    (fun _ => Prop)
+    (fun (n:nat) => False)
+    (fun sym l tf => tf)
+    True
+    (fun _ _ => and)
+    t
+.
+
+Lemma vterm_is_closed_implies_vterm_is_not_var
+    {Σ : spec_syntax.Signature}
+    (t : VTerm.term Σ)
+    : vterm_is_closed t -> forall v, t <> Var v
+.
+Proof.
+    intros H1 v H2.
+    subst t.
+    simpl in H1.
+    exact H1.
+Qed.
+
+Definition closed_vterm_proj_sym
+    {Σ : spec_syntax.Signature}
+    ( ct : { t : VTerm.term Σ | vterm_is_closed t })
+    : VSignature.symbol (m2c_sig Σ)
+:=
+let t := `ct in
+match inspect t with
+| @exist _ _ (Var v) pfeq =>
+    match vterm_is_closed_implies_vterm_is_not_var t (proj2_sig ct) v pfeq with
+    end
+| @exist _ _ (Fun s _) _ => s
+end
+.
+
+Definition closed_vterm_proj_args0
+    {Σ : spec_syntax.Signature}
+    ( ct : { t : VTerm.term Σ | vterm_is_closed t })
+    : list (VTerm.term Σ)
+:=
+let t := `ct in
+match inspect t with
+| @exist _ _ (Var v) pfeq =>
+    match vterm_is_closed_implies_vterm_is_not_var t (proj2_sig ct) v pfeq with
+    end
+| @exist _ _ (Fun _ args) _ => args
+end
+.
+
+Lemma closed_vterm_proj_args0_closed
+    {Σ : spec_syntax.Signature}
+    ( ct : { t : VTerm.term Σ | vterm_is_closed t })
+    : Forall vterm_is_closed (closed_vterm_proj_args0 ct)
+.
+Proof.
+    rewrite (sig_eta ct).
+    remember (proj2_sig ct) as pf.
+    clear Heqpf.
+    remember (`ct) as t.
+    clear Heqt ct.
+
+    destruct t.
+    {
+        cbn in pf.
+        inversion pf.
+    }
+    cbn.
+    induction l.
+    {
+        apply Forall_nil.
+    }
+    {
+        cbn in pf.
+        destruct pf as [pf1 pf2].
+        apply Forall_cons.
+        {
+            apply pf1.
+        }
+        {
+            apply IHl.
+            apply pf2.
+        }
+    }
+Qed.
+
+Lemma vterm_is_closed_Fun
+    {Σ : spec_syntax.Signature}
+    s
+    (l: list (term Σ)) :
+    Forall vterm_is_closed l ->
+    @vterm_is_closed Σ (@VTerm.Fun Σ s l)
+.
+Proof.
+    intros H.
+    induction l; cbn.
+    { exact I. }
+    {
+        inversion H; subst; clear H.
+        ltac1:(naive_solver).
+    }
+Qed.
+
+Program Fixpoint m2c_AppliedOperator'_symbol_builtin
+    {Σ : spec_syntax.Signature}
+    (g : AppliedOperator' spec_syntax.symbol builtin_value)
+    : { t : VTerm.term Σ | vterm_is_closed t }
+:=
+match g with
+| ao_operator s => @exist _ _ (@VTerm.Fun Σ (c_sym_symbol Σ s) []) _
+| ao_app_operand aps b =>
+    let tpf : { t : VTerm.term Σ | vterm_is_closed t }
+        := m2c_AppliedOperator'_symbol_builtin aps in
+    let sym : symbol Σ
+        := closed_vterm_proj_sym tpf in
+    let args : list (VTerm.term Σ)
+        := closed_vterm_proj_args0 tpf in
+    let pf
+        := closed_vterm_proj_args0_closed tpf in
+    let b'
+        := (@VTerm.Fun Σ (c_sym_builtin_value Σ b) []) in
+    let args'
+        := (args ++ [b']) in
+    @exist _ _ 
+        (@VTerm.Fun Σ sym args')
+        (@vterm_is_closed_Fun Σ sym args'
+            (Forall_app_2 vterm_is_closed args [b'] pf
+                (Forall_cons vterm_is_closed b' [] _ (Forall_nil vterm_is_closed))
+            )
+        )
+| ao_app_ao aps1 aps2 =>
+    let tpf1 : { t : VTerm.term Σ | vterm_is_closed t }
+        := m2c_AppliedOperator'_symbol_builtin aps1 in
+    let tpf2 : { t : VTerm.term Σ | vterm_is_closed t }
+        := m2c_AppliedOperator'_symbol_builtin aps2 in
+    let sym : symbol Σ
+        := closed_vterm_proj_sym tpf1 in
+    let args : list (VTerm.term Σ)
+        := closed_vterm_proj_args0 tpf1 in
+    let pf
+        := closed_vterm_proj_args0_closed tpf1 in
+    @exist _ _
+        (@VTerm.Fun Σ sym (args ++ [`tpf2]))
+        (@vterm_is_closed_Fun Σ sym (args ++ [`tpf2])
+            (Forall_app_2 vterm_is_closed args [`tpf2]
+                (closed_vterm_proj_args0_closed _)
+                _
+            )
+        )
+end
+.
+
